tracing out A in 3 qubit system added

PartialTraceDefinitions.v
@@ -109,3 +109,172 @@ by_cell.
     reflexivity.
 }
 Qed.
+
+Definition partial_trace_3q_a (M: Square 8): Square 4 :=
+    fun x y =>
+    match (x,y) with
+    | (0,0) => (M 0 0)%nat + (M 4 4)%nat
+    | (0,1) => (M 0 1)%nat + (M 4 5)%nat
+    | (0,2) => (M 0 2)%nat + (M 4 6)%nat
+    | (0,3) => (M 0 3)%nat + (M 4 7)%nat
+    | (1,0) => (M 1 0)%nat + (M 5 4)%nat
+    | (1,1) => (M 1 1)%nat + (M 5 5)%nat
+    | (1,2) => (M 1 2)%nat + (M 5 6)%nat
+    | (1,3) => (M 1 3)%nat + (M 5 7)%nat
+    | (2,0) => (M 2 0)%nat + (M 6 4)%nat
+    | (2,1) => (M 2 1)%nat + (M 6 5)%nat
+    | (2,2) => (M 2 2)%nat + (M 6 6)%nat
+    | (2,3) => (M 2 3)%nat + (M 6 7)%nat
+    | (3,0) => (M 3 0)%nat + (M 7 4)%nat
+    | (3,1) => (M 3 1)%nat + (M 7 5)%nat
+    | (3,2) => (M 3 2)%nat + (M 7 6)%nat
+    | (3,3) => (M 3 3)%nat + (M 7 7)%nat
+    | _ => C0
+    end.
+
+Lemma WF_partial_trace_3q_a : forall (A : Square 8),
+    WF_Matrix (partial_trace_3q_a A).
+Proof.
+unfold WF_Matrix.
+intros.
+destruct H.
+{
+    unfold partial_trace_3q_a.
+    destruct x as [|x'].
+    contradict H.
+    lia.
+    destruct x' as [|x''].
+    contradict H.
+    lia.
+    destruct x'' as [|x'''].
+    contradict H.
+    lia.
+    destruct x''' as [|x''''].
+    contradict H.
+    lia.
+    reflexivity.
+}
+{
+    unfold partial_trace_3q_a.
+    destruct x as [|x'].
+    {
+        destruct y as [|y'].
+        contradict H.
+        lia.
+        destruct y' as [|y''].
+        contradict H.
+        lia.
+        destruct y'' as [|y'''].
+        contradict H.
+        lia.
+        destruct y''' as [|y''''].
+        contradict H.
+        lia.
+        reflexivity.
+    }
+    destruct x' as [|x''].
+    { 
+        destruct y as [|y'].
+        contradict H.
+        lia.
+        destruct y' as [|y''].
+        contradict H.
+        lia.
+        destruct y'' as [|y'''].
+        contradict H.
+        lia.
+        destruct y''' as [|y''''].
+        contradict H.
+        lia.
+        reflexivity.
+    }
+    destruct x'' as [|x'''].
+    { 
+        destruct y as [|y'].
+        contradict H.
+        lia.
+        destruct y' as [|y''].
+        contradict H.
+        lia.
+        destruct y'' as [|y'''].
+        contradict H.
+        lia.
+        destruct y''' as [|y''''].
+        contradict H.
+        lia.
+        reflexivity.
+    }
+    destruct x''' as [|x''''].
+    { 
+        destruct y as [|y'].
+        contradict H.
+        lia.
+        destruct y' as [|y''].
+        contradict H.
+        lia.
+        destruct y'' as [|y'''].
+        contradict H.
+        lia.
+        destruct y''' as [|y''''].
+        contradict H.
+        lia.
+        reflexivity.
+    }
+    reflexivity.
+}
+Qed.
+
+Lemma partial_trace_3q_a_linear : forall (c:C) (A B : Square 4),
+  partial_trace_3q_a (A .+ c .* B) = partial_trace_3q_a A .+ c .* partial_trace_3q_a B.
+Proof.
+intros.
+apply mat_equiv_eq.
+apply WF_partial_trace_3q_a.
+apply WF_plus.
+apply WF_partial_trace_3q_a.
+apply WF_scale.
+apply WF_partial_trace_3q_a.
+by_cell.
+unfold partial_trace_3q_a; unfold scale; unfold Mplus. lca.
+unfold partial_trace_3q_a; unfold scale; unfold Mplus. lca.
+unfold partial_trace_3q_a; unfold scale; unfold Mplus. lca.
+unfold partial_trace_3q_a; unfold scale; unfold Mplus. lca.
+unfold partial_trace_3q_a; unfold scale; unfold Mplus. lca.
+unfold partial_trace_3q_a; unfold scale; unfold Mplus. lca.
+unfold partial_trace_3q_a; unfold scale; unfold Mplus. lca.
+unfold partial_trace_3q_a; unfold scale; unfold Mplus. lca.
+unfold partial_trace_3q_a; unfold scale; unfold Mplus. lca.
+unfold partial_trace_3q_a; unfold scale; unfold Mplus. lca.
+unfold partial_trace_3q_a; unfold scale; unfold Mplus. lca.
+unfold partial_trace_3q_a; unfold scale; unfold Mplus. lca.
+unfold partial_trace_3q_a; unfold scale; unfold Mplus. lca.
+unfold partial_trace_3q_a; unfold scale; unfold Mplus. lca.
+unfold partial_trace_3q_a; unfold scale; unfold Mplus. lca.
+unfold partial_trace_3q_a; unfold scale; unfold Mplus. lca.
+Qed.
+
+Lemma partial_trace_3q_a_compat : forall (A B : Square 4),
+  A = B -> partial_trace_3q_a A = partial_trace_3q_a B.
+Proof.
+intros.
+apply mat_equiv_eq.
+apply WF_partial_trace_3q_a.
+apply WF_partial_trace_3q_a.
+by_cell.
+unfold partial_trace_3q_a. rewrite H. reflexivity.
+unfold partial_trace_3q_a. rewrite H. reflexivity.
+unfold partial_trace_3q_a. rewrite H. reflexivity.
+unfold partial_trace_3q_a. rewrite H. reflexivity.
+unfold partial_trace_3q_a. rewrite H. reflexivity.
+unfold partial_trace_3q_a. rewrite H. reflexivity.
+unfold partial_trace_3q_a. rewrite H. reflexivity.
+unfold partial_trace_3q_a. rewrite H. reflexivity.
+unfold partial_trace_3q_a. rewrite H. reflexivity.
+unfold partial_trace_3q_a. rewrite H. reflexivity.
+unfold partial_trace_3q_a. rewrite H. reflexivity.
+unfold partial_trace_3q_a. rewrite H. reflexivity.
+unfold partial_trace_3q_a. rewrite H. reflexivity.
+unfold partial_trace_3q_a. rewrite H. reflexivity.
+unfold partial_trace_3q_a. rewrite H. reflexivity.
+unfold partial_trace_3q_a. rewrite H. reflexivity.
+Qed.
